LwRust/Extractor/CompleteProgram.lean
@@ -84,6 +84,7 @@ syntax (name := ctermMove) "move" clval : cterm
 syntax (name := ctermCopy) "copy" clval : cterm
 syntax (name := ctermEq) cterm "==" cterm : cterm
 syntax (name := ctermIte) "if" cterm cterm "else" cterm : cterm
+syntax (name := ctermWhile) "while" term cterm cterm : cterm
 
 /-!
 Checked constructor annotations for the generator.
@@ -161,6 +162,9 @@ abbrev ctermEq_ctor (lhs rhs : Term) : Term :=
 
 abbrev ctermIte_ctor (condition trueBranch falseBranch : Term) : Term :=
   show Term from (.ite condition trueBranch falseBranch)
+
+abbrev ctermWhile_ctor (bodyLifetime : Lifetime) (condition body : Term) : Term :=
+  show Term from (.whileLoop bodyLifetime condition body)
 
 end SyntaxCtor
 
