LwRust/Extractor/Generated/PartialProgram.lean
@@ -87,6 +87,9 @@ inductive PartialTerm where
   | iteCondition (condition : PartialTerm)
   | iteTrueBranch (condition : Term) (trueBranch : PartialTerm)
   | iteFalseBranch (condition : Term) (trueBranch : Term) (falseBranch : PartialTerm)
+  -- derived from: SyntaxCtor.ctermWhile_ctor {bodyLifetime} {condition} {body}
+  | whileCondition (bodyLifetime : Lifetime) (condition : PartialTerm)
+  | whileBody (bodyLifetime : Lifetime) (condition : Term) (body : PartialTerm)
   -- derived from: SyntaxCtor.ctermBlock_ctor {lifetime} {terms}
   | blockStart
   -- derived from: SyntaxCtor.ctermLetMut_ctor {name} {initialiser}
@@ -103,6 +106,8 @@ inductive PartialTerm where
   | copyStart
   -- derived from: SyntaxCtor.ctermIte_ctor {condition} {trueBranch} {falseBranch}
   | iteStart
+  -- derived from: SyntaxCtor.ctermWhile_ctor {bodyLifetime} {condition} {body}
+  | whileStart
   deriving Repr
 
 end
@@ -253,6 +258,13 @@ inductive CompletesTerm : PartialTerm → Term → Prop where
   | ctermIte_iteFalseBranch {condition : Term} {trueBranch : Term} {falseBranch : PartialTerm} {falseBranch' : Term} :
       CompletesTerm falseBranch falseBranch' →
       CompletesTerm (PartialTerm.iteFalseBranch condition trueBranch falseBranch) (SyntaxCtor.ctermIte_ctor condition trueBranch falseBranch')
+  -- derived from: SyntaxCtor.ctermWhile_ctor {bodyLifetime} {condition} {body}
+  | ctermWhile_whileCondition {bodyLifetime : Lifetime} {condition : PartialTerm} {condition' : Term} {body : Term} :
+      CompletesTerm condition condition' →
+      CompletesTerm (PartialTerm.whileCondition bodyLifetime condition) (SyntaxCtor.ctermWhile_ctor bodyLifetime condition' body)
+  | ctermWhile_whileBody {bodyLifetime : Lifetime} {condition : Term} {body : PartialTerm} {body' : Term} :
+      CompletesTerm body body' →
+      CompletesTerm (PartialTerm.whileBody bodyLifetime condition body) (SyntaxCtor.ctermWhile_ctor bodyLifetime condition body')
   -- derived from: SyntaxCtor.ctermBlock_ctor {lifetime} {terms}
   | ctermBlock_blockStart {lifetime : Lifetime} {terms : List Term} :
       CompletesTerm (PartialTerm.blockStart) (SyntaxCtor.ctermBlock_ctor lifetime terms)
@@ -279,6 +291,9 @@ inductive CompletesTerm : PartialTerm → Term → Prop where
   -- derived from: SyntaxCtor.ctermIte_ctor {condition} {trueBranch} {falseBranch}
   | ctermIte_iteStart {condition : Term} {trueBranch : Term} {falseBranch : Term} :
       CompletesTerm (PartialTerm.iteStart) (SyntaxCtor.ctermIte_ctor condition trueBranch falseBranch)
+  -- derived from: SyntaxCtor.ctermWhile_ctor {bodyLifetime} {condition} {body}
+  | ctermWhile_whileStart {bodyLifetime : Lifetime} {condition : Term} {body : Term} :
+      CompletesTerm (PartialTerm.whileStart) (SyntaxCtor.ctermWhile_ctor bodyLifetime condition body)
 
 end
 
